Kore bool theory - negation axioms

kore/src/theories/Bool.v
@@ -1,3 +1,5 @@
+(* From Equations Require Import Equations. *)
+From MatchingLogic Require Export stdpp_ext.
 From Kore Require Export Semantics.
 Import Signature.StringVariables.
 Import Kore.Syntax.Notations.
@@ -67,42 +69,105 @@ Module BoolSyntax.
   |}.
 
   Open Scope hlist_scope.
-  Definition Kbool_theory : @Theory BoolSignature :=
+  Open Scope string_scope.
+
+(*
+dv is only used with the following parameters:
+\dv{SortBool{}}("true")
+\dv{SortBool{}}("false")
+\dv{SortInt{}}("n") (n is a number)
+\dv{SortString{}}("s") (s is a string)
+\dv{SortKConfigVar{}}("$PGM")
+
+  axiom{R} \implies{R} (
+    \and{R}(
+      \top{R}(),
+      \and{R} (
+          \in{SortBool{}, R} (
+            X0:SortBool{},
+            \dv{SortBool{}}("false")
+          ),
+          \top{R} ()
+        )),
+    \equals{SortBool{},R} (
+      LblnotBool'Unds'{}(X0:SortBool{}),
+     \and{SortBool{}} (
+       \dv{SortBool{}}("true"),
+        \top{SortBool{}}())))
+
+  axiom{R} \implies{R} (
+    \and{R}(
+      \top{R}(),
+      \and{R} (
+          \in{SortBool{}, R} (
+            X0:SortBool{},
+            \dv{SortBool{}}("true")
+          ),
+          \top{R} ()
+        )),
+    \equals{SortBool{},R} (
+      LblnotBool'Unds'{}(X0:SortBool{}),
+     \and{SortBool{}} (
+       \dv{SortBool{}}("false"),
+        \top{SortBool{}}())))
+
+  axiom{R} \implies{R} (
+    \and{R}(
+      \top{R}(),
+      \and{R} (
+          \in{SortBool{}, R} (
+            X0:SortBool{},
+            \and{SortBool{}}(\dv{SortBool{}}("false"),Var'Unds'Gen1:SortBool{})
+          ),\and{R} (
+          \in{SortBool{}, R} (
+            X1:SortBool{},
+            Var'Unds'Gen0:SortBool{}
+          ),
+          \top{R} ()
+        ))),
+    \equals{SortBool{},R} (
+      Lbl'Unds'andBool'Unds'{}(X0:SortBool{},X1:SortBool{}),
+     \and{SortBool{}} (
+       Var'Unds'Gen1:SortBool{},
+        \top{SortBool{}}())))
+ *)
+
+  Program Definition Kbool_theory : @Theory BoolSignature :=
     PropSet (fun pat =>
-      exists R, pat = existT R (KnotBool ⋅ ⟨Ktrue ⋅ ⟨⟩⟩ =k{R} Ktrue ⋅ ⟨⟩)
-    ).
+      (exists R, pat =                              (* v-- this should be dv *)
+        existT R ((Top{R} and kore_fevar "X" ⊆k{R} Kfalse ⋅ ⟨⟩)
+          --->                               (* v-- this should be dv *)
+         (KnotBool ⋅ ⟨kore_fevar "X"⟩ =k{R} (Ktrue ⋅ ⟨⟩ and Top{Kbool})))
+      ) \/
+      (exists R, pat =
+        existT R ((Top{R} and kore_fevar "X" ⊆k{R} Ktrue ⋅ ⟨⟩)
+          --->
+        (KnotBool ⋅ ⟨kore_fevar "X"⟩ =k{R} (Kfalse ⋅ ⟨⟩ and Top{Kbool})))
+      ) \/
+      (exists R, pat =
+        existT R ((Top{R} and
+                   kore_fevar "X0" ⊆k{R} (Kfalse ⋅ ⟨⟩ and kore_fevar "_") and
+                   @kore_fevar _ _ _ Kbool "X1" ⊆k{R} kore_fevar "_" and
+                   Top{R})
+          --->
+        (KandBool ⋅ ⟨kore_fevar "X0"; kore_fevar "X1"⟩ =k{R} (kore_fevar "_" and Top{Kbool})))
+      )
+      (* \/ For testing:
+      pat = existT Kbool Top{Kbool} *)
+    )
+    .
+    (* Sometimes, implicit arguments are needed, e.g. if X ⊆ Y, and X and Y are both free variables. However, this might be resolved if X and Y would be bound *)
 
 End BoolSyntax.
+
+(* Tactic Notation "deconstruct_elem_of_Theory" :=
+  repeat match goal with
+  | [ H : _ ∈ ?Γ |- _ ] => destruct H
+  end; (* clear; *) simpl. *)
 
 Module BoolSemantics.
 
   Import BoolSyntax.
-
-  (* Definition bool_carrier (s : Ksorts) :=
-    match s with 
-    | Kbool => bool
-    end.
-  Check hlist.
-  Program Definition bool_app
-    (σ : Ksyms)
-    (l : hlist bool_carrier (arg_sorts σ)) :
-      propset (bool_carrier (ret_sort σ)) :=
-  match σ with
-  | Ktrue => {[true]}
-  | Kfalse => {[false]}
-  | KnotBool => _
-  | KandBool => _
-  | KandThenBool => _
-  | KxorBool => _
-  | KorBool => _
-  | KorElseBool => _
-  | KimpliesBool => _
-  end. *)
-
-  (* Program Definition BoolModel : @Model BoolSignature := {|
-    carrier := bool_carrier;
-    app := bool_app;
-  |}. *)
 
   Definition BoolModel : @Model BoolSignature :=
     mkModel_singleton
@@ -118,16 +183,56 @@ Module BoolSemantics.
                     implb)
       ltac:(intros []; auto with typeclass_instances).
 
+  Ltac unfold_elem_of :=
+  match goal with
+  | [H : _ ∈ _ |- _]  => destruct H
+  end.
+
+(*   Lemma Propset_full_or_empty :
+    forall (A : Type) (P : Prop),
+      {[_ : A | P]} = ⊤ \/
+      {[_ : A | P]} = ∅.
+  Proof.
+    intros.
+    Require Import ClassicalPropType.
+    pose proof ClassicalProp.classic.
+  Admitted. *)
+
+  Lemma propset_difference_neg :
+    forall {A : Type} (P : A -> Prop),
+      ⊤ ∖ {[x : A | P x]} = {[x : A | ~P x]}.
+  Proof.
+    intros.
+    set_solver.
+  Qed.
+
   Goal satT Kbool_theory BoolModel.
   Proof.
-    unfold satT. intros.
-    
-    cbn. unfold op_all, op_not. intros.
-    deconstruct_elem_of_Theory; eval_helper; set_helper.
-    now rewrite_singleton_all.
+    (* unfold sat defs *)
+    unfold satT, satM. intros.
 
-    repeat (unfold bevar_subst, Equality.block, solution_left, eq_rect_r; simpl).
-    eval_helper. set_helper. now rewrite_singleton_all.
+    (* Generate a goal for each axiom: *)
+    unfold Kbool_theory in H.
+    unfold_elem_of; destruct_or?; destruct_ex?; subst.
+
+    (* simplification *)
+    * simpl.
+      eval_helper.
+      unshelve (repeat erewrite app_ext_singleton).
+      1-3: simpl; try repeat econstructor. (* This seems to be fragile *)
+      cbn.
+      
+      
+      
+      
+      Search propset ⊤ ∅.
+      
+       set_solver.
+    
+    
+    
+    set_helper.
+    rewrite_singleton_all. cbn. reflexivity.
   Qed.
 
 End BoolSemantics.
